automatic induction; see the end of unit1.ver and the proof of progress in stlc.fst

src/absyn/const.fs
@@ -47,46 +47,43 @@ let kbin k1 k2 k'            = mk_Kind_arrow([Inl (null_bvar k1), false;
 let ktern k1 k2 k3 k'        = mk_Kind_arrow([Inl (null_bvar k1), false; 
                                               Inl (null_bvar k2), false;
                                               Inl (null_bvar k3), false], k') dummyRange
-let true_lid = pconst "True"
-let false_lid = pconst "False"
-let and_lid = pconst "l_and"  
-let or_lid = pconst "l_or"    
-let not_lid = pconst "l_not"  
-let lbl_lid = pconst "LBL"    
-let imp_lid = pconst "l_imp"
-let iff_lid = pconst "l_iff"      
-let ite_lid = pconst "ITE" 
+let true_lid   = pconst "True"
+let false_lid  = pconst "False"
+let and_lid    = pconst "l_and"  
+let or_lid     = pconst "l_or"    
+let not_lid    = pconst "l_not"  
+let lbl_lid    = pconst "LBL"    
+let imp_lid    = pconst "l_imp"
+let iff_lid    = pconst "l_iff"      
+let ite_lid    = pconst "ITE" 
 let exists_lid = pconst "Exists"  
 let forall_lid = pconst "Forall"  
 let exTyp_lid  = pconst "ExistsTyp"
 let allTyp_lid = pconst "ForallTyp"
-let b2t_lid = pconst "b2t" (* coercion from boolean to type *)
+let b2t_lid    = pconst "b2t" (* coercion from boolean to type *)
+let using_IH   = pconst "InductionHyp"
 
-(* Predicates corresponding to binops *)
-let eq_lid    = pconst  "Eq"
-let eq2_lid   = pconst  "Eq2"
-let eqA_lid   = pconst  "EqA"
-let eqT_lid   = pconst  "EqTyp"
-let neq_lid   = pconst  "neq"
-let neq2_lid  = pconst  "neq2"
-
-(* Common logical functions for various theories *)
-let typeof_lid = pconst "TypeOf" 
-let kindof_lid = pconst "KindOf" 
+(* Various equality predicates *)
+let eq_lid     = pconst  "Eq"
+let eq2_lid    = pconst  "Eq2"
+let eqA_lid    = pconst  "EqA"
+let eqT_lid    = pconst  "EqTyp"
+let neq_lid    = pconst  "neq"
+let neq2_lid   = pconst  "neq2"
 
 (* Some common term constructors *)
-let exp_true_bool  = mk_Exp_constant (Const_bool true) tun dummyRange
-let exp_false_bool = mk_Exp_constant (Const_bool false) tun dummyRange
-let exp_unit       = mk_Exp_constant (Const_unit) tun dummyRange
-let cons_lid       = pconst  "Cons"
-let nil_lid        = pconst  "Nil"
-let ref_lid        = pconst  "ref"
-let assume_lid     = pconst  "Assume"
-let assert_lid     = pconst  "Assert"
-let pipe_right_lid = pconst "pipe_right"
-let pipe_left_lid  = pconst "pipe_left"
+let exp_true_bool   = mk_Exp_constant (Const_bool true) tun dummyRange
+let exp_false_bool  = mk_Exp_constant (Const_bool false) tun dummyRange
+let exp_unit        = mk_Exp_constant (Const_unit) tun dummyRange
+let cons_lid        = pconst  "Cons"
+let nil_lid         = pconst  "Nil"
+let ref_lid         = pconst  "ref"
+let assume_lid      = pconst  "Assume"
+let assert_lid      = pconst  "Assert"
+let pipe_right_lid  = pconst "pipe_right"
+let pipe_left_lid   = pconst "pipe_left"
 let list_append_lid = p2l ["List"; "append"]
-let strcat_lid     = p2l ["String"; "strcat"]
+let strcat_lid      = p2l ["String"; "strcat"]
 
 (* Primitive operators *)
 let op_Eq              = pconst "op_Equality"
